\begin{exercise}
	Let
	$$
		f(x,y) = \sin(\pi xy) \cdot e^{-\frac{x}{3}} \quad \text{and} \quad p = \left(1, \frac{1}{3}\right).
	$$
	\begin{enumerate}
		\item Compute $\nabla f$ and $(\nabla f)(p)$. Use the special values of $\sin$ and $\cos$.
		\item Find the directions of maximum increase and decrease at $p$. You can give approximate values.
		\item Give the direction of the contour line at $p$.
		\item The equation of the tangent plane of the graph of $f$ at $(x_0, y_0)$ is
		      $$
			      z = f(x_0, y_0) + (\nabla f)(x_0, y_0) \cdot (x - x_0, y - y_0).
		      $$
		      Determine the equation of the tangent plane of $z = f(x,y)$ at $p$. Give a normal vector of the plane.
		\item Find the directional derivative of $f(x,y)$ at $p$ along the vector
		      $$
			      v = \frac{1}{\sqrt{2}} (1,1).
		      $$
	\end{enumerate}
\end{exercise}

\begin{solution}
	\begin{enumerate}
		\item
		      $$
			      \begin{aligned}
				      \frac{\partial f}{\partial x} & = e^{-x/3} \left( \pi y \cos(\pi xy) - \frac{1}{3} \sin(\pi xy) \right) \\
				      \frac{\partial f}{\partial y} & = e^{-x/3} \pi x \cos(\pi xy)
			      \end{aligned}
		      $$
		      $$
			      \begin{aligned}
				      \implies (\nabla f)(x,y) & = \left( \frac{\partial f}{\partial x}, \frac{\partial f}{\partial y} \right)                  \\
				                               & = e^{-x/3} \left( \pi y \cos(\pi xy) - \frac{1}{3} \sin(\pi xy), \; \pi x \cos(\pi xy) \right)
			      \end{aligned}
		      $$
		      With $\sin(\frac{\pi}{3}) = \frac{\sqrt{3}}{2}$ and $\cos(\frac{\pi}{3}) = \frac{1}{2}$:
		      $$
			      (\nabla f)(p) = e^{-1/3} \left( \frac{\pi - \sqrt{3}}{6}, \; \frac{\pi}{2} \right)
		      $$
		\item
		      Maximum increase: $(\nabla f)(p)$, maximum decrease: $-(\nabla f)(p)$
		\item
		      Contour lines are perpendicular to the gradient:
		      $$
			      (x, \; y) \cdot (-y, \; x) = 0 \implies u = e^{-1/3} \left( - \frac{\pi}{2}, \; \frac{\pi - \sqrt{3}}{6} \right)
		      $$
		\item
		      $$
			      \begin{aligned}
				      z = f(x, y) & = f(p) + (\nabla f)(p) \cdot (x - 1, y - \frac{1}{3})                                                                                \\
				                  & = \frac{\sqrt{3}}{2} e^{-1/3} + e^{-1/3} \left( \frac{\pi - \sqrt{3}}{6}, \; \frac{\pi}{2} \right) \cdot (x - 1, \; y - \frac{1}{3}) \\
				                  & = e^{-1/3} \left( \frac{\sqrt{3}}{2} + \frac{1}{6} \left( (\pi - \sqrt{3}) x + 3 \pi y + \sqrt{3} \right) \right)
			      \end{aligned}
		      $$
		      The surface $z = f(x, y)$ can be written as $F(x, y, z) = f(x, y) - z = 0$. Therefore,
		      $$
			      \nabla F = (f_x, \; f_y, \; -1)
		      $$
		      is normal to the surface:
		      $$
			      \begin{aligned}
				      n := (\nabla F)(p) & = \left( f_x(p), \; f_y(p), \; -1\right)                                            \\
				                         & = \left( \frac{\pi - \sqrt{3}}{6} e^{-1/3}, \; \frac{\pi}{2} e^{-1/3},\; -1 \right)
			      \end{aligned}
		      $$
		\item
		      $$
			      \begin{aligned}
				      (\nabla f)(p) \cdot v & = e^{-1/3} \left( \frac{\pi - \sqrt{3}}{6}, \; \frac{\pi}{2} \right) \cdot \frac{1}{\sqrt{2}} (1,1) \\
				                            & = \frac{e^{-1/3}}{\sqrt{2}} \left( \frac{\pi - \sqrt{3}}{6} + \frac{\pi}{2} \right)                 \\
				                            & = \frac{e^{-1/3}}{\sqrt{2}} \cdot \frac{4\pi - \sqrt{3}}{6}
			      \end{aligned}
		      $$
	\end{enumerate}
\end{solution}
