\begin{exercise}
	Let
	$$
		f(x,y,z) = x^2 y z^3 \quad \text{and} \quad F(x,y,z) = (xz, -y^2, 2x^2 y).
	$$
	Give $\nabla f$, $\nabla^2 f$, $\nabla \cdot F$, and $\nabla \times F$.
\end{exercise}

\begin{solution}
	$$
		\begin{aligned}
			\nabla f       & = \left( \frac{\partial f}{\partial x},\; \frac{\partial f}{\partial y},\; \frac{\partial f}{\partial z} \right) \\
			               & = \left( 2x y z^3,\; x^2 z^3,\; 3x^2 y z^2 \right)                                                               \\[1em]
			\nabla^2 f     & = \frac{\partial^2 f}{\partial x^2} + \frac{\partial^2 f}{\partial y^2} + \frac{\partial^2 f}{\partial z^2}      \\
			               & = 2y z^3 + 0 + 6x^2 y z                                                                                          \\
			               & = 2y z^3 + 6x^2 y z                                                                                              \\[1em]
			\nabla \cdot F & = \frac{\partial}{\partial x}(xz) + \frac{\partial}{\partial y}(-y^2) + \frac{\partial}{\partial z}(2x^2 y)      \\
			               & = z - 2y                                                                                                         \\[1em]
		\end{aligned}
	$$
	$$
		\begin{aligned}
			\frac{\partial F_x}{\partial y} & = \frac{\partial}{\partial y} (xz) = 0            \\
			\frac{\partial F_x}{\partial z} & = \frac{\partial}{\partial z} (xz) = x            \\
			\frac{\partial F_y}{\partial x} & = \frac{\partial}{\partial x} (-y^{2}) = 0        \\
			\frac{\partial F_y}{\partial z} & = \frac{\partial}{\partial z} (-y^{2}) = 0        \\
			\frac{\partial F_z}{\partial x} & = \frac{\partial}{\partial x} (2x^{2}y)  = 4xy    \\
			\frac{\partial F_z}{\partial y} & = \frac{\partial}{\partial y} (2x^{2}y)  = 2x^{2}
		\end{aligned}
	$$
	$$
		\begin{aligned}
			\nabla \times F & = \left(
			\frac{\partial F_z}{\partial y} - \frac{\partial F_y}{\partial z},\;
			\frac{\partial F_x}{\partial z} - \frac{\partial F_z}{\partial x},\;
			\frac{\partial F_y}{\partial x} - \frac{\partial F_x}{\partial y}
			\right)                                                           \\
			                & = \left( 2x^{2} - 0,\; x - 4xy,\; 0 - 0 \right) \\
			                & = \left( 2x^{2},\; x - 4xy,\; 0 \right)         \\
		\end{aligned}
	$$
\end{solution}
