\begin{exercise}
	Compute differential forms:
	\begin{enumerate}
		\item Let
		      $$
			      f(x,y,z) = \frac{x}{yz}
		      $$
		      be a scalar function. Give the differential form $df$.
		      \newline \emph{Hint:}
		      $$
			      df = F_1(x,y,z) \, dx + F_2(x,y,z) \, dy + F_3(x,y,z) \, dz.
		      $$
		\item Let
		      $$
			      \omega = x^2 \sin(y) \, dx + 2^x \cos(y) \, dy
		      $$
		      be a differential form on $\R^2$. Give the 2-form $d\omega$.
		      \newline \emph{Hint:}
		      $$
			      d\omega = \phi(x,y) \, dx \wedge dy.
		      $$
		\item Let
		      $$
			      \omega = x^2 \sin(y) \, dx + z^2 \cos(y) \, dy - xy^2 \, dz
		      $$
		      be a differential form on $\R^3$. Give the 2-form $d\omega$.
		      \newline \emph{Hint:}
		      $$
			      d\omega = F_1(x,y,z) \, dy \wedge dz + F_2(x,y,z) \, dz \wedge dx + F_3(x,y,z) \, dx \wedge dy.
		      $$
	\end{enumerate}
\end{exercise}

\begin{solution}
	\begin{enumerate}
		\item
		      $$
			      df = \frac{1}{yz} \, dx - \frac{x}{y^2z} \, dy - \frac{x}{yz^2} \, dz
		      $$
		\item
		      $$
			      \begin{aligned}
				      \phi(x, y) & = \frac{\partial}{\partial x}(2^x \cos(y)) - \frac{\partial}{\partial y}(x^2 \sin(y)) \\
				                 & = \ln(2) 2^x \cos(y) - x^2 \cos(y)                                                    \\
				                 & = \cos(y) \left( \ln(2) 2^x - x^2 \right)                                             \\
			      \end{aligned}
		      $$
		      So:
		      $$
			      \begin{aligned}
				      d\omega & = \phi(x,y) \, dx \wedge dy                                              \\
				              & = \left( \cos(y) \left( \ln(2) 2^x - x^2 \right) \right) \, dx \wedge dy
			      \end{aligned}
		      $$
		\item
		      $$
			      \begin{aligned}
				      F_1(x,y,z) & = \frac{\partial}{\partial y}(-xy^2) - \frac{\partial}{\partial z}(z^2 \cos y) = -2xy - 2z \cos y                  \\
				      F_2(x,y,z) & = \frac{\partial}{\partial z}(x^2 \sin y) - \frac{\partial}{\partial x}(-xy^2) = 0 + y^2 = y^2                     \\
				      F_3(x,y,z) & = \frac{\partial}{\partial x}(z^2 \cos y) - \frac{\partial}{\partial y}(x^2 \sin y) = 0 - x^2 \cos y = -x^2 \cos y
			      \end{aligned}
		      $$
		      So:
		      $$
			      d\omega = (-2xy - 2z \cos y) \, dy \wedge dz + y^2 \, dz \wedge dx - (x^2 \cos y) \, dx \wedge dy.
		      $$
	\end{enumerate}
\end{solution}
