\section{25-40}

\begin{exercise}
	Let $f$ be the scalar function defined by $f(x,y) = xy$. Sketch the contour lines and the vector field $\nabla f$.
\end{exercise}

\begin{solution}
	$$
		(\nabla f)(x,y) = \left( \frac{\partial f}{\partial x}, \frac{\partial f}{\partial y} \right) = (y,x)
	$$
	\begin{center}
		\begin{tikzpicture}
			\begin{axis}[
					axis equal,
					xlabel=$x$,
					ylabel=$y$,
					domain=-3:3,
					y domain=-3:3,
					view={0}{90},
					enlargelimits=false,
					axis on top,
					colorbar,
					colormap/viridis,
				]
				\addplot3[
					contour gnuplot={levels={-4,-2,-1,-0.5,0,0.5,1,2,4},labels=false},
					thick,
					samples=50,
				] {x*y};
				\addplot3[
					quiver={
							u={y},
							v={x},
							scale arrows=0.15,
						},
					-stealth,
					samples=15,
				] {0};
			\end{axis}
		\end{tikzpicture}
	\end{center}
\end{solution}

\begin{exercise}
	Let
	$$
		f(x,y) = \sin(\pi xy) \cdot e^{-\frac{x}{3}} \quad \text{and} \quad p = \left(1, \frac{1}{3}\right).
	$$
	\begin{enumerate}
		\item Compute $\nabla f$ and $(\nabla f)(p)$. Use the special values of $\sin$ and $\cos$.
		\item Find the directions of maximum increase and decrease at $p$. You can give approximate values.
		\item Give the direction of the contour line at $p$.
		\item The equation of the tangent plane of the graph of $f$ at $(x_0, y_0)$ is
		      $$
			      z = f(x_0, y_0) + (\nabla f)(x_0, y_0) \cdot (x - x_0, y - y_0).
		      $$
		      Determine the equation of the tangent plane of $z = f(x,y)$ at $p$. Give a normal vector of the plane.
		\item Find the directional derivative of $f(x,y)$ at $p$ along the vector
		      $$
			      v = \frac{1}{\sqrt{2}} (1,1).
		      $$
	\end{enumerate}
\end{exercise}

\begin{solution}
	\begin{enumerate}
		\item
		      $$
			      \begin{aligned}
				      \frac{\partial f}{\partial x} & = e^{-x/3} \left( \pi y \cos(\pi xy) - \frac{1}{3} \sin(\pi xy) \right) \\
				      \frac{\partial f}{\partial y} & = e^{-x/3} \pi x \cos(\pi xy)
			      \end{aligned}
		      $$
		      $$
			      \begin{aligned}
				      \implies (\nabla f)(x,y) & = \left( \frac{\partial f}{\partial x}, \frac{\partial f}{\partial y} \right)                  \\
				                               & = e^{-x/3} \left( \pi y \cos(\pi xy) - \frac{1}{3} \sin(\pi xy), \; \pi x \cos(\pi xy) \right)
			      \end{aligned}
		      $$
		      With $\sin(\frac{\pi}{3}) = \frac{\sqrt{3}}{2}$ and $\cos(\frac{\pi}{3}) = \frac{1}{2}$:
		      $$
			      (\nabla f)(p) = e^{-1/3} \left( \frac{\pi - \sqrt{3}}{6}, \; \frac{\pi}{2} \right)
		      $$
		\item
		      Maximum increase: $(\nabla f)(p)$, maximum decrease: $-(\nabla f)(p)$
		\item
		      Contour lines are perpendicular to the gradient:
		      $$
			      (x, \; y) \cdot (-y, \; x) = 0 \implies u = e^{-1/3} \left( - \frac{\pi}{2}, \; \frac{\pi - \sqrt{3}}{6} \right)
		      $$
		\item
		      $$
			      \begin{aligned}
				      z = f(x, y) & = f(p) + (\nabla f)(p) \cdot (x - 1, y - \frac{1}{3})                                                                                \\
				                  & = \frac{\sqrt{3}}{2} e^{-1/3} + e^{-1/3} \left( \frac{\pi - \sqrt{3}}{6}, \; \frac{\pi}{2} \right) \cdot (x - 1, \; y - \frac{1}{3}) \\
				                  & = e^{-1/3} \left( \frac{\sqrt{3}}{2} + \frac{1}{6} \left( (\pi - \sqrt{3}) x + 3 \pi y + \sqrt{3} \right) \right)
			      \end{aligned}
		      $$
		      The surface $z = f(x, y)$ can be written as $F(x, y, z) = f(x, y) - z = 0$. Therefore,
		      $$
			      \nabla F = (f_x, \; f_y, \; -1)
		      $$
		      is normal to the surface:
		      $$
			      \begin{aligned}
				      n := (\nabla F)(p) & = \left( f_x(p), \; f_y(p), \; -1\right)                                            \\
				                         & = \left( \frac{\pi - \sqrt{3}}{6} e^{-1/3}, \; \frac{\pi}{2} e^{-1/3},\; -1 \right)
			      \end{aligned}
		      $$
		\item
		      $$
			      \begin{aligned}
				      (\nabla f)(p) \cdot v & = e^{-1/3} \left( \frac{\pi - \sqrt{3}}{6}, \; \frac{\pi}{2} \right) \cdot \frac{1}{\sqrt{2}} (1,1) \\
				                            & = \frac{e^{-1/3}}{\sqrt{2}} \left( \frac{\pi - \sqrt{3}}{6} + \frac{\pi}{2} \right)                 \\
				                            & = \frac{e^{-1/3}}{\sqrt{2}} \cdot \frac{4\pi - \sqrt{3}}{6}
			      \end{aligned}
		      $$
	\end{enumerate}
\end{solution}

\begin{exercise}
	Compute curl and divergence of the vector field
	$$
		F(x,y,z) = (\sin(x)xy, \, ze^{-x}, \, yz).
	$$
\end{exercise}

\begin{solution}
	$$
		\begin{aligned}
			\frac{\partial F_x}{\partial y} & = \frac{\partial}{\partial y} (\sin(x) xy) = x \sin(x) \\
			\frac{\partial F_x}{\partial z} & = \frac{\partial}{\partial z} (\sin(x) xy) = 0         \\
			\frac{\partial F_y}{\partial x} & = \frac{\partial}{\partial x} (ze^{-x}) = -ze^{-x}     \\
			\frac{\partial F_y}{\partial z} & = \frac{\partial}{\partial z} (ze^{-x}) = e^{-x}       \\
			\frac{\partial F_z}{\partial x} & = \frac{\partial}{\partial x} (yz)  = 0                \\
			\frac{\partial F_z}{\partial y} & = \frac{\partial}{\partial y} (yz)  = z
		\end{aligned}
	$$
	$$
		\begin{aligned}
			\text{curl}\, F = \nabla \times F & = \left(
			\frac{\partial F_z}{\partial y} - \frac{\partial F_y}{\partial z},\;
			\frac{\partial F_x}{\partial z} - \frac{\partial F_z}{\partial x},\;
			\frac{\partial F_y}{\partial x} - \frac{\partial F_x}{\partial y}
			\right)                                                                                         \\
			                                  & = \left( z - e^{-x},\; 0 - 0,\; -ze^{-x} - x\sin(x) \right) \\
			                                  & = \left( z - e^{-x},\; 0,\; -ze^{-x} - x\sin(x) \right)     \\[1em]
		\end{aligned}
	$$
	$$
		\begin{aligned}
			\text{div}\, F = \nabla \cdot F & = \frac{\partial F_x}{\partial x} + \frac{\partial F_y}{\partial y} + \frac{\partial F_z}{\partial z}                             \\
			                                & = \frac{\partial}{\partial x}\big(\sin(x)xy\big) + \frac{\partial}{\partial y}\big(ze^{-x}\big) + \frac{\partial}{\partial z}(yz) \\
			                                & = y\sin(x) + xy\cos(x) + 0 + y                                                                                                    \\
			                                & = y\sin(x) + xy\cos(x) + y
		\end{aligned}
	$$
\end{solution}

\begin{exercise}
	Let
	$$
		f(x,y,z) = x^2 y z^3 \quad \text{and} \quad F(x,y,z) = (xz, -y^2, 2x^2 y).
	$$
	Give $\nabla f$, $\nabla^2 f$, $\nabla \cdot F$, and $\nabla \times F$.
\end{exercise}

\begin{solution}
	$$
		\begin{aligned}
			\nabla f       & = \left( \frac{\partial f}{\partial x},\; \frac{\partial f}{\partial y},\; \frac{\partial f}{\partial z} \right) \\
			               & = \left( 2x y z^3,\; x^2 z^3,\; 3x^2 y z^2 \right)                                                               \\[1em]
			\nabla^2 f     & = \frac{\partial^2 f}{\partial x^2} + \frac{\partial^2 f}{\partial y^2} + \frac{\partial^2 f}{\partial z^2}      \\
			               & = 2y z^3 + 0 + 6x^2 y z                                                                                          \\
			               & = 2y z^3 + 6x^2 y z                                                                                              \\[1em]
			\nabla \cdot F & = \frac{\partial}{\partial x}(xz) + \frac{\partial}{\partial y}(-y^2) + \frac{\partial}{\partial z}(2x^2 y)      \\
			               & = z - 2y                                                                                                         \\[1em]
		\end{aligned}
	$$
	$$
		\begin{aligned}
			\frac{\partial F_x}{\partial y} & = \frac{\partial}{\partial y} (xz) = 0            \\
			\frac{\partial F_x}{\partial z} & = \frac{\partial}{\partial z} (xz) = x            \\
			\frac{\partial F_y}{\partial x} & = \frac{\partial}{\partial x} (-y^{2}) = 0        \\
			\frac{\partial F_y}{\partial z} & = \frac{\partial}{\partial z} (-y^{2}) = 0        \\
			\frac{\partial F_z}{\partial x} & = \frac{\partial}{\partial x} (2x^{2}y)  = 4xy    \\
			\frac{\partial F_z}{\partial y} & = \frac{\partial}{\partial y} (2x^{2}y)  = 2x^{2}
		\end{aligned}
	$$
	$$
		\begin{aligned}
			\nabla \times F & = \left(
			\frac{\partial F_z}{\partial y} - \frac{\partial F_y}{\partial z},\;
			\frac{\partial F_x}{\partial z} - \frac{\partial F_z}{\partial x},\;
			\frac{\partial F_y}{\partial x} - \frac{\partial F_x}{\partial y}
			\right)                                                           \\
			                & = \left( 2x^{2} - 0,\; x - 4xy,\; 0 - 0 \right) \\
			                & = \left( 2x^{2},\; x - 4xy,\; 0 \right)         \\
		\end{aligned}
	$$
\end{solution}

\begin{exercise}
	Compute differential forms:
	\begin{enumerate}
		\item Let
		      $$
			      f(x,y,z) = \frac{x}{yz}
		      $$
		      be a scalar function. Give the differential form $df$.
		      \newline \emph{Hint:}
		      $$
			      df = F_1(x,y,z) \, dx + F_2(x,y,z) \, dy + F_3(x,y,z) \, dz.
		      $$
		\item Let
		      $$
			      \omega = x^2 \sin(y) \, dx + 2^x \cos(y) \, dy
		      $$
		      be a differential form on $\R^2$. Give the 2-form $d\omega$.
		      \newline \emph{Hint:}
		      $$
			      d\omega = \phi(x,y) \, dx \wedge dy.
		      $$
		\item Let
		      $$
			      \omega = x^2 \sin(y) \, dx + z^2 \cos(y) \, dy - xy^2 \, dz
		      $$
		      be a differential form on $\R^3$. Give the 2-form $d\omega$.
		      \newline \emph{Hint:}
		      $$
			      d\omega = F_1(x,y,z) \, dy \wedge dz + F_2(x,y,z) \, dz \wedge dx + F_3(x,y,z) \, dx \wedge dy.
		      $$
	\end{enumerate}
\end{exercise}

\begin{solution}
	\begin{enumerate}
		\item
		      $$
			      df = \frac{1}{yz} \, dx - \frac{x}{y^2z} \, dy - \frac{x}{yz^2} \, dz
		      $$
		\item
		      $$
			      \begin{aligned}
				      \phi(x, y) & = \frac{\partial}{\partial x}(2^x \cos(y)) - \frac{\partial}{\partial y}(x^2 \sin(y)) \\
				                 & = \ln(2) 2^x \cos(y) - x^2 \cos(y)                                                    \\
				                 & = \cos(y) \left( \ln(2) 2^x - x^2 \right)                                             \\
			      \end{aligned}
		      $$
		      So:
		      $$
			      \begin{aligned}
				      d\omega & = \phi(x,y) \, dx \wedge dy                                              \\
				              & = \left( \cos(y) \left( \ln(2) 2^x - x^2 \right) \right) \, dx \wedge dy
			      \end{aligned}
		      $$
		\item
		      $$
			      \begin{aligned}
				      F_1(x,y,z) & = \frac{\partial}{\partial y}(-xy^2) - \frac{\partial}{\partial z}(z^2 \cos y) = -2xy - 2z \cos y                  \\
				      F_2(x,y,z) & = \frac{\partial}{\partial z}(x^2 \sin y) - \frac{\partial}{\partial x}(-xy^2) = 0 + y^2 = y^2                     \\
				      F_3(x,y,z) & = \frac{\partial}{\partial x}(z^2 \cos y) - \frac{\partial}{\partial y}(x^2 \sin y) = 0 - x^2 \cos y = -x^2 \cos y
			      \end{aligned}
		      $$
		      So:
		      $$
			      d\omega = (-2xy - 2z \cos y) \, dy \wedge dz + y^2 \, dz \wedge dx - (x^2 \cos y) \, dx \wedge dy.
		      $$
	\end{enumerate}
\end{solution}
